challenge_response.v
@@ -175,7 +175,7 @@ iIntros "#? #? #ctx inv #d_kA #d_kB Hpost".
 iPoseProof "ctx" as "(? & ? & ?)".
 wp_pures. wp_bind (mknonce _).
 iApply (wp_mknonce (λ _, True)%I (λ _, True)%I) => //.
-iIntros (nA) "_ #p_nA _ unreg".
+iIntros (nA) "_ _ #p_nA _ unreg".
 rewrite (term_token_difference _ (↑N)) //.
 iDestruct "unreg" as "[unreg _]".
 iAssert (public nA) as "{p_nA} p_nA"; first by iApply "p_nA".
@@ -243,7 +243,7 @@ case: (bool_decide_reflect (_ = repr_key_type Dec)); last protocol_failure.
 case: kt=> // _.
 wp_pures; wp_bind (mknonce _).
 iApply (wp_mknonce (λ _, True)%I (λ _, True)%I) => //.
-iIntros (nB) "_ #p_nB _ unreg".
+iIntros (nB) "_ _ #p_nB _ unreg".
 rewrite (term_token_difference _ (↑N)) //.
 iDestruct "unreg" as "[token _]".
 iAssert (public nB) as "{p_nB} HnB"; first by iApply "p_nB".
