examples/permanent.v
@@ -114,8 +114,8 @@ Definition game : val := λ: "mkchan",
 
   (* Generate signature keys and publicize verification key *)
   let: "k"   := mksigkey #() in
-  let: "sk"  := Fst "k" in
-  let: "vk"  := Snd "k" in
+  let: "sk"  := key Enc "k" in
+  let: "vk"  := key Dec "k" in
   send "c" "vk" ;;
 
   (* Initialize server state *)
@@ -147,6 +147,9 @@ iIntros "!> %c #cP". wp_pures.
 (* Generate server key. Keep the signing key secret. *)
 wp_bind (mksigkey _). iApply (wp_mksigkey with "[//] hon phase") => //.
 iIntros (k) "#p_vk #hon' phase".
+wp_pures.
+wp_apply wp_key. wp_pures.
+wp_apply wp_key. wp_pures.
 iMod (phase_auth_discard with "phase") as "#phase".
 (* Publicize verification key. *)
 wp_pures. wp_bind (send _ _). iApply wp_send => //. wp_pures.
