tls13.v
@@ -661,7 +661,7 @@ Proof.
 iIntros "#? #p_ke post"; rewrite /I.new; wp_pures.
 iApply Meth.wp_case; case: ke => [psk|g|psk g]; wp_pures.
 - wp_bind (mknonce _); iApply (wp_mknonce (λ _, True)%I (λ _, True)%I) => //.
-  iIntros (cn) "_ #p_cn _ token"; wp_list; wp_term_of_list.
+  iIntros (cn) "_ _ #p_cn _ token"; wp_list; wp_term_of_list.
   wp_tag.
   iApply ("post" $! (Psk psk cn) with "[] [] token") => //=.
   do !iSplit => //.
@@ -671,7 +671,7 @@ iApply Meth.wp_case; case: ke => [psk|g|psk g]; wp_pures.
   { by iApply public_minted. }
   iIntros (a) "_ #p_a _"; wp_list.
   wp_bind (mknonce _); iApply (wp_mknonce (λ _, True)%I (λ _, True)%I) => //.
-  iIntros (cn) "_ #p_cn _ token"; wp_list; wp_term_of_list.
+  iIntros (cn) "_ _ #p_cn _ token"; wp_list; wp_term_of_list.
   wp_tag.
   rewrite (term_token_difference _ ⊤); try set_solver.
   iDestruct "token" as "[token _]".
@@ -683,7 +683,7 @@ iApply Meth.wp_case; case: ke => [psk|g|psk g]; wp_pures.
   { by iApply public_minted. }
   iIntros (a) "_ #p_a _"; wp_list.
   wp_bind (mknonce _); iApply (wp_mknonce (λ _, True)%I (λ _, True)%I) => //.
-  iIntros (cn) "_ #p_cn _ token"; wp_list; wp_term_of_list.
+  iIntros (cn) "_ _ #p_cn _ token"; wp_list; wp_term_of_list.
   wp_tag.
   iApply ("post" $! (PskDh psk g cn a)) => //=.
   do !iSplit => //.
@@ -1185,7 +1185,7 @@ iApply CShare.wp_case.
 case: ke => [psk' cn|g' cn gx|psk' g' cn gx] /= in e_check *; wp_pures.
 - subst psk.
   wp_bind (mknonce _); iApply (wp_mknonce (λ _, True)%I (λ _, True)%I) => //.
-  iIntros (a) "_ #pred_a _ token"; wp_list; wp_term_of_list.
+  iIntros (a) "_ _ #pred_a _ token"; wp_list; wp_term_of_list.
   wp_tag; iModIntro.
   iApply ("post" $! (Psk _ _ a)) => //=.
   rewrite public_tag public_of_list /=.
@@ -1197,7 +1197,7 @@ case: ke => [psk' cn|g' cn gx|psk' g' cn gx] /= in e_check *; wp_pures.
   { by iApply public_minted. }
   iIntros (a) "_ #pred_a _"; wp_list.
   wp_bind (mknonce _); iApply (wp_mknonce (λ _, True)%I (λ _, True)%I) => //.
-  iIntros (sn) "_ #p_sn _ token"; wp_list; wp_term_of_list.
+  iIntros (sn) "_ _ #p_sn _ token"; wp_list; wp_term_of_list.
   wp_tag; iModIntro.
   iApply ("post" $! (Dh g cn sn gx a)) => //=.
   rewrite !public_tag !public_of_list /=.
@@ -1209,7 +1209,7 @@ case: ke => [psk' cn|g' cn gx|psk' g' cn gx] /= in e_check *; wp_pures.
   { by iApply public_minted. }
   iIntros (a) "_ #pred_a _"; wp_list.
   wp_bind (mknonce _); iApply (wp_mknonce (λ _, True)%I (λ _, True)%I) => //.
-  iIntros (sn) "_ #p_sn _ token"; wp_list; wp_term_of_list.
+  iIntros (sn) "_ _ #p_sn _ token"; wp_list; wp_term_of_list.
   wp_tag; iModIntro.
   iApply ("post" $! (PskDh _ g cn sn gx a)) => //.
   rewrite !public_tag !public_of_list /=.
